src/DeadLock.v
@@ -1,3 +1,4 @@
+Require Import Io.All.
 Require Choose.
 Require Model.
 Require Trace.
@@ -11,10 +12,26 @@ Module NotStuck.
 End NotStuck.
 
 Module Choose.
-  Module DeadLockFree.
+  (*Module DeadLockFree.
     Definition t {E S} (m : Model.t E S) (s : S) {A} (x : t E A) : Prop :=
       forall trace s' x', Steps.t x trace -> NotStuck.t m s trace s' x' ->
       exists trace', exists s'', exists v,
         LastSteps.t x' trace' /\ NotStuck.t m s' trace s'' v.
-  End DeadLockFree.
+  End DeadLockFree.*)
 End Choose.
+
+Module C.
+  (*Module DeadLockFree.
+    Definition t {E S} (m : Model.t E S) (s : S) {A} (x : C.t E A) : Prop :=
+      forall trace s' x', Steps.t x trace -> NotStuck.t m s trace s' x' ->
+      exists trace', exists s'', exists v,
+        LastSteps.t x' trace' /\ NotStuck.t m s' trace s'' v.
+  End DeadLockFree.
+
+  Lemma dead_lock {E S} (m : Model.t E S) (s : S) {A} (x : C.t E A)
+    (H : Choose.DeadLockFree.t m s (compile x)) : DeadLockFree.t m s x.
+    intros trace s' x' H_trace H_not_stuck.
+    Check H _ _ _ (traces _ _ H_trace).
+    exists
+  Qed.*)
+End C.
